Basic/Tree.v
@@ -3,6 +3,9 @@ Add Rec LoadPath "/home/zeimer/Code/Coq".
 Require Export LinDec.
 Require Export RCCBase.
 
+Require Import HSLib.Control.Functor.
+Require Import HSLib.Control.Foldable.
+
 Inductive Tree (A : Type) : Type :=
     | E : Tree A
     | T : A -> list (Tree A) -> Tree A.
@@ -10,6 +13,40 @@ Inductive Tree (A : Type) : Type :=
 Arguments E [A].
 Arguments T [A] _ _.
 
+Inductive elem {A : Type} (x : A) : Tree A -> Prop :=
+    | elem0 : forall l : list (Tree A), elem x (T x l)
+    | elem1 : forall (a : A) (l : list (Tree A)),
+        Exists (fun t => elem x t) l -> elem x (T a l).
+
+Inductive elem' {A : Type} (x : A) : Tree A -> Prop :=
+    | elem0' : forall l : list (Tree A), elem' x (T x l)
+    | elem1' :
+        forall (a : A) (t : Tree A) (ts : list (Tree A)),
+          elem' x t -> elem' x (T a (t :: ts))
+    | elem2' :
+        forall (a : A) (t : Tree A) (ts : list (Tree A)),
+          elem' x (T a ts) -> elem' x (T a (t :: ts)). 
+
+Inductive isHeap {A : LinDec} : Tree A -> Prop :=
+    | isHeap_E : isHeap E
+    | isHeap_T :
+        forall (v : A) (l : list (Tree A)),
+          Forall (fun t : Tree A => forall x : A, elem x t -> v ≤ x) l ->
+          Forall (fun t : Tree A => isHeap t) l ->
+            isHeap (T v l).
+
+Hint Constructors elem elem' isHeap.
+
+Hint Extern 0 =>
+match goal with
+    | |- ~ elem _ E => intro
+    | |- ~ elem' _ E => intro
+    | H : elem _ E |- _ => inv H
+    | H : elem' _ E |- _ => inv H
+    | H : Exists _ [] |- _ => inv H
+end.
+
+(** * Induction principles *)
 Fixpoint Tree_rect'
   (A : Type) (P : Tree A -> Type) (Q : list (Tree A) -> Type)
   (HE : P E)
@@ -65,39 +102,6 @@ Proof.
       apply HT; assumption.
 Qed.
 
-Inductive elem {A : Type} (x : A) : Tree A -> Prop :=
-    | elem0 : forall l : list (Tree A), elem x (T x l)
-    | elem1 : forall (a : A) (l : list (Tree A)),
-        Exists (fun t => elem x t) l -> elem x (T a l).
-
-Inductive elem' {A : Type} (x : A) : Tree A -> Prop :=
-    | elem0' : forall l : list (Tree A), elem' x (T x l)
-    | elem1' :
-        forall (a : A) (t : Tree A) (ts : list (Tree A)),
-          elem' x t -> elem' x (T a (t :: ts))
-    | elem2' :
-        forall (a : A) (t : Tree A) (ts : list (Tree A)),
-          elem' x (T a ts) -> elem' x (T a (t :: ts)). 
-
-Inductive isHeap {A : LinDec} : Tree A -> Prop :=
-    | isHeap_E : isHeap E
-    | isHeap_T :
-        forall (v : A) (l : list (Tree A)),
-          Forall (fun t : Tree A => forall x : A, elem x t -> v ≤ x) l ->
-          Forall (fun t : Tree A => isHeap t) l ->
-            isHeap (T v l).
-
-Hint Constructors elem isHeap.
-
-Require Import HSLib.Control.Functor.
-
-Fixpoint fmap_Tree
-  {A B : Type} (f : A -> B) (t : Tree A) : Tree B :=
-match t with
-    | E => E
-    | T x l => T (f x) (map (fmap_Tree f) l)
-end.
-
 Ltac Tree_ind :=
 repeat match goal with
     | |- forall t' : Tree _, _ =>
@@ -107,9 +111,16 @@ repeat match goal with
         let IHt := fresh "IHt" in
         let IHts := fresh "IHts" in
           induction t' as [| x | x t ts IHt IHts] using Tree_ind_proper2;
-          cbn in *; try reflexivity; f_equal; rewrite ?IHt; auto;
-          try (inv IHts; fail)
+          cbn in *; intros; try reflexivity; f_equal; rewrite ?IHt;
+          rewrite ?id_eq; try (inv IHts; fail); auto; try congruence
     | |- forall _, _ => intro
+end.
+
+Fixpoint fmap_Tree
+  {A B : Type} (f : A -> B) (t : Tree A) : Tree B :=
+match t with
+    | E => E
+    | T x l => T (f x) (map (fmap_Tree f) l)
 end.
 
 Instance Functor_Tree : Functor Tree :=
@@ -117,68 +128,8 @@ Instance Functor_Tree : Functor Tree :=
     fmap := @fmap_Tree
 }.
 Proof.
-  all: intros; ext t.
-    destruct t as [| x t] using Tree_ind_proper; cbn.
-      reflexivity.
-      induction H; cbn.
-        reflexivity.
-        rewrite !id_eq in *. f_equal. inv IHForall.
-    destruct t as [| x t] using Tree_ind_proper; cbn.
-      reflexivity.
-      induction H; cbn.
-        reflexivity.
-        f_equal. inv IHForall. rewrite H2. f_equal. assumption.
-Restart.
-  all: intros; ext t.
-    induction t as [| x | x t ts] using Tree_ind_proper2;
-    cbn in *; rewrite !id_eq in *; try reflexivity.
-      rewrite IHt. inv IHt0.
-    induction t as [| x | x t ts] using Tree_ind_proper2;
-    cbn in *; try reflexivity.
-      rewrite IHt. inv IHt0.
-Restart.
   all: intros; ext t; gen t; Tree_ind.
-    rewrite !id_eq. inv IHts.
 Defined.
-
-Fixpoint size {A : Type} (t : Tree A) : nat :=
-match t with
-    | E => 0
-    | T _ ts => 1 + fold_right (fun h t => size h + t) 0 ts
-end.
-
-Lemma fmap_size :
-  forall (A B : Type) (f : A -> B) (t : Tree A),
-    size (fmap_Tree f t) = size t.
-Proof.
-  Tree_ind.
-Qed.
-
-Hint Constructors elem'.
-
-Hint Extern 0 =>
-match goal with
-    | H : elem' _ E |- _ => inv H
-end.
-
-Lemma fmap_elem' :
-  forall (A B : Type) (f : A -> B) (t : Tree A) (x : A),
-    elem' x t -> elem' (f x) (fmap_Tree f t).
-Proof.
-  induction 1; cbn; auto.
-Qed.
-
-(*Lemma fmap_elem :
-  forall (A B : Type) (f : A -> B) (t : Tree A) (x : A),
-    elem x t -> elem (f x) (fmap_Tree f t).
-Proof.
-  induction 1; cbn; auto.
-    induction H. cbn.
-Qed.*)
-
-Require Import HSLib.Control.Foldable.
-
-Print Foldable.
 
 Fixpoint foldMap_Tree
   {A : Type} {M : Monoid} (f : A -> M) (t : Tree A) : M :=
@@ -186,12 +137,6 @@ match t with
     | E => neutr
     | T x l => op (f x)
                   (fold_right (fun h t => op (foldMap_Tree f h) t) neutr l)
-        (*let aux := fix aux (l : list (Tree A)) : M :=
-        match l with
-            | [] => neutr
-            | t :: ts => op (foldMap_Tree f t) (aux ts)
-        end
-        in op (f x) (aux l)*)
 end.
 
 Instance Foldable_Tree : Foldable Tree :=
@@ -213,4 +158,113 @@ Proof.
         rewrite IHt. reflexivity.
 Defined.
 
-Check size.
+(** * Utility functions *)
+
+(*Fixpoint foldr {A B : Type} (f : A -> B -> B) (b : B) (t : Tree A) : B :=
+match t with
+    | E => b
+    | T x ts => f x (fold_right (fun t ts => foldr f ts t) b ts)
+end.
+
+Fixpoint foldr' {A B : Type} (f : A -> B -> B) (b : B) (t : Tree A) : B :=
+match t with
+    | E => b
+    | T x ts =>
+        let
+          aux := fix aux (b : B) (ts : list (Tree A)) : B :=
+          match ts with
+              | [] => f x b
+              | t :: ts' =>
+                  let b' := foldr f b t in aux b' ts'
+          end
+        in aux b ts
+end.
+
+Lemma foldr_foldr' : @foldr = @foldr'.
+Proof.
+  ext A; ext  B; ext f; ext b; ext t; gen b; gen t. Tree_ind.
+  rewrite IHt. rewrite <- IHts. f_equal.
+  rewrite <- !IHt.
+Abort.
+
+Definition foldr2
+  {A B : Type} (f : A -> list B -> B) (b : B) (t : Tree A) : B :=
+match t with
+    | E => b
+    | T x ts => f x (map foldr2 *)
+
+(* TODO Definition sizef {A : Type} (t : Tree A) : nat :=
+  foldr (fun _ ts => 1 + ts) 0 t.
+
+Lemma sizef_spec : @sizef = @size.
+Proof.
+  ext A; ext t; gen t. Tree_ind. inv IHts.
+Abort.
+
+Definition sizef' {A : Type} (t : Tree A) : nat :=
+  foldr' (fun _ => S) 0 t.
+
+Compute sizef (T 5 [T 0 []; T 1 []]).
+Compute sizef' (T 5 [T 0 []; T 1 []]).
+
+Check @foldr (list (Tree nat)) nat. (fun ts t => T 0 (t :: ts)) E.
+
+ (T 5 [T 0 []; T 1 []]).
+Compute sizef' (T 5 [T 0 []; T 1 []]). *)
+
+Definition isEmpty
+  {A : Type} (t : Tree A) : bool :=
+match t with
+    | E => true
+    | _ => false
+end.
+
+Fixpoint size {A : Type} (t : Tree A) : nat :=
+match t with
+    | E => 0
+    | T _ ts => 1 + fold_right (fun h t => size h + t) 0 ts
+end.
+
+Fixpoint countTree {A : LinDec} (x : A) (t : Tree A) : nat :=
+match t with
+    | E => 0
+    | T x' l =>
+        (if x =? x' then S else id)
+          (fold_right (fun h t => countTree x h + t) 0 l)
+end.
+
+(** Properties of [isEmpty]. *)
+
+Lemma isEmpty_elem :
+  forall (A : Type) (x : A) (t : Tree A),
+    isEmpty t = true -> ~ elem x t.
+Proof. Tree_ind. Qed.
+
+Lemma isEmpty_isHeap :
+  forall (A : LinDec) (t : Tree A),
+    isEmpty t = true -> isHeap t.
+Proof. Tree_ind. Qed.
+
+Lemma isEmpty_size_false :
+  forall (A : Type) (t : Tree A),
+    isEmpty t = false -> size t <> 0.
+Proof. Tree_ind. Qed.
+
+Lemma isEmpty_size_true :
+  forall (A : LinDec) (t : Tree A),
+    isEmpty t = true -> size t = 0.
+Proof. Tree_ind. Qed.
+
+(** Properties of [size]. *)
+
+Lemma size_fmap :
+  forall (A B : Type) (f : A -> B) (t : Tree A),
+    size (fmap_Tree f t) = size t.
+Proof. Tree_ind. Qed.
+
+Lemma fmap_elem' :
+  forall (A B : Type) (f : A -> B) (t : Tree A) (x : A),
+    elem' x t -> elem' (f x) (fmap_Tree f t).
+Proof.
+  induction 1; cbn; auto.
+Qed.
