ADT/Deque.v
@@ -1,0 +1,139 @@
+Add Rec LoadPath "/home/zeimer/Code/Coq".
+
+Require Import RCCBase.
+
+Module Type Deque.
+
+Parameter Deque : Type -> Type.
+
+Parameter empty :
+  forall {A : Type}, Deque A.
+
+Parameter isEmpty :
+  forall {A : Type}, Deque A -> bool.
+
+Parameter cons :
+  forall {A : Type}, A -> Deque A -> Deque A.
+
+Parameter head :
+  forall {A : Type}, Deque A -> option A.
+
+Parameter tail :
+  forall {A : Type}, Deque A -> option (Deque A).
+
+Parameter snoc :
+  forall {A : Type}, A -> Deque A -> Deque A.
+
+Parameter last :
+  forall {A : Type}, Deque A -> option A.
+
+Parameter init :
+  forall {A : Type}, Deque A -> option (Deque A).
+
+(* Properties of [isEmpty]. *)
+Parameter isEmpty_empty :
+  forall A : Type, isEmpty (@empty A) = true.
+
+Parameter isEmpty_cons :
+  forall (A : Type) (x : A) (d : Deque A),
+    isEmpty (cons x d) = false.
+
+Parameter isEmpty_head_true :
+  forall (A : Type) (d : Deque A),
+    isEmpty d = true (*TODO: <*)-> head d = None.
+
+Parameter isEmpty_head_false :
+  forall (A : Type) (d : Deque A),
+    isEmpty d = false <-> exists h : A, head d = Some h.
+
+Parameter isEmpty_tail_false :
+  forall (A : Type) (d : Deque A),
+    isEmpty d = false <-> exists d' : Deque A, tail d = Some d'.
+
+Parameter isEmpty_tail_true :
+  forall (A : Type) (d : Deque A),
+    isEmpty d = true <-> tail d = None.
+
+Parameter isEmpty_snoc :
+  forall (A : Type) (x : A) (d : Deque A),
+    isEmpty (snoc x d) = false.
+
+Parameter isEmpty_last_true :
+  forall (A : Type) (d : Deque A),
+    isEmpty d = true (*TODO: <*)-> last d = None.
+
+Parameter isEmpty_last_false :
+  forall (A : Type) (d : Deque A),
+    isEmpty d = false <-> exists h : A, last d = Some h.
+
+Parameter isEmpty_init_false :
+  forall (A : Type) (d : Deque A),
+    isEmpty d = false <-> exists d' : Deque A, init d = Some d'.
+
+Parameter isEmpty_init_true :
+  forall (A : Type) (d : Deque A),
+    isEmpty d = true <-> init d = None.
+
+(* Properties of [head]. *)
+Parameter head_empty :
+  forall A : Type, head (@empty A) = None.
+
+Parameter head_cons :
+  forall (A : Type) (x : A) (d : Deque A),
+    head (cons x d) = Some x.
+
+Parameter head_snoc_false :
+  forall (A : Type) (x : A) (d : Deque A),
+    isEmpty d = false -> head (snoc x d) = head d.
+
+Parameter head_snoc_true :
+  forall (A : Type) (x : A) (d : Deque A),
+    isEmpty d = true -> head (snoc x d) = Some x.
+
+(* Properties of [last]. *)
+Parameter last_empty :
+  forall A : Type, last (@empty A) = None.
+
+Parameter last_snoc :
+  forall (A : Type) (x : A) (d : Deque A),
+    last (snoc x d) = Some x.
+
+Parameter last_cons_false :
+  forall (A : Type) (x : A) (d : Deque A),
+    isEmpty d = false -> last (cons x d) = last d.
+
+Parameter last_cons_true :
+  forall (A : Type) (x : A) (d : Deque A),
+    isEmpty d = true -> last (cons x d) = Some x.
+
+(* Properties of [tail]. *)
+Parameter tail_empty :
+  forall A : Type, tail (@empty A) = None.
+
+Parameter tail_cons :
+  forall (A : Type) (x : A) (d : Deque A),
+    tail (cons x d) = Some d.
+
+(*Require Import HSLib.Instances.Option.
+
+Parameter tail_snoc :
+  forall (A : Type) (x : A) (d : Deque A),
+    isEmpty d = false -> tail (snoc x d) = fmap_Option (snoc x) (tail d).*)
+
+(* Properties of [init]. *)
+Parameter init_empty :
+  forall A : Type, init (@empty A) = None.
+
+Parameter init_snoc :
+  forall (A : Type) (x : A) (d : Deque A),
+    init (snoc x d) = Some d.
+
+(*Parameter init_cons :
+  forall (A : Type) (x : A) (d : Deque A),
+    isEmpty d = false -> init (cons x d) = fmap_Option (cons x) (init d).*)
+
+
+(*Hint Rewrite isEmpty_empty isEmpty_snoc last_empty last_singl
+             tail_empty tail_singl : Deque.*)
+
+End Deque.
